All but sanity builds - latter should be easy.

holsrcs/class_infoScript.sml
@@ -20,155 +20,298 @@ open statesTheory aggregatesTheory
 val _ = new_theory "class_info";
 
 val is_class_name_def = Define`
-  is_class_name st (nns, nm) =
-    ~(nns.idents = []) /\
-    case LAST nns.idents of
-       CName s -> (nns with idents updated_by FRONT, s) IN FDOM st.classmap
-    || _ -> F
+  is_class_name st cppid = cppid IN FDOM st.classmap
 `;
 
+val tempid_inst_def = Define`
+  (tempid_inst sigma (TemplateConstant tn) = TemplateConstant tn) /\
+  (tempid_inst sigma (TemplateVar s) =
+     case FINDL (\ (p,a). p = TTemp (TemplateVar s)) sigma of
+        NONE -> TemplateVar s
+     || SOME (p, a) -> (case a of TTemp x -> x))
+`
+
 (* instantiate a type with template arguments *)
-val type_inst_def = Define`
-  (type_inst sigma (TypeName cspec) = cspec_inst sigma cspec) /\
+val type_inst_defn = Hol_defn "type_inst" `
+  (type_inst sigma (TypeID cid) = cppid_ty_inst sigma cid) /\
   (type_inst sigma (Ptr ty) = Ptr (type_inst sigma ty)) /\
   (type_inst sigma (MPtr nm ty) =
-      MPtr (dest_class (cspec_inst sigma nm)) (type_inst sigma ty)) /\
-  (type_inst sigma (Ref ty) = Ref (type_inst sigma ta)) /\
+      MPtr (cppid_inst sigma nm) (type_inst sigma ty)) /\
+  (type_inst sigma (Ref ty) = Ref (type_inst sigma ty)) /\
   (type_inst sigma (Array ty n) = Array (type_inst sigma ty) n) /\
   (type_inst sigma (Function ty tylist) =
       Function (type_inst sigma ty) (MAP (type_inst sigma) tylist)) /\
   (type_inst sigma (Const ty) = Const (type_inst sigma ty)) /\
+  (type_inst sigma (Class cid) = Class (cppid_inst sigma cid)) /\
   (type_inst sigma ty = ty)
 
     /\
 
   (* instantiates what is really a name, but returns it as a class type *)
-  (cspec_inst sigma (nns, cnm) =
-     if nns.absolute then
-       Class (nns_inst sigma nns, cnm_temparg_only_inst sigma cnm)
-     else if nns.idents = [] then
-       Class (nns, SND (dest_class (cname_inst sigma cnm)))
-     else let outer = HD nns.idents in
-          let rest0 = TL nns.idents in
-          let rest = MAP (cnm_temparg_only_inst sigma) rest0
-          in
-            Class
-              (<| idents := SND (dest_class (cname_inst sigma outer)) :: rest;
-                  absolute := F |>,
-               cnm_temparg_only_inst sigma cnm))
-
-     /\
-
-  (* likewise, returns an instantiated name as a type *)
-  (cname_inst sigma (CName s) =
-     case FINDL (\ (p,a). p = TempType s) sigma of
-        NONE -> Class (Base (CName s))
-     || SOME (p, a) -> (case a of TType ty -> ty || x2 -> ARB)) /\
-  (cname_inst sigma (TempCall temp args0) =
-     let args = MAP (temparg_inst sigma) args0
-     in
-         Class (Base (TempCall (tempname_inst sigma temp) args)))
-
-     /\
-
-  (tempname_inst sigma (nns, tempnm) =
-       (* don't need to instantiate nns here because it can't include
-          any template applications: templates can't return templates, and
-          the name we're looking at is a template call *)
-       if nns.absolute \/ ~(nns.idents = []) then (nns,tempnm)
-       else
-         case FINDL (\ (p,a). ?argtys. p = TempTemp tempnm argtys) sigma of
-          NONE -> (nns,tempnm)
-       || SOME (p, a) -> case a of TTemp tynm -> tynm || x3 -> ARB)
-
-     /\
-
-   (cnm_temparg_only_inst sigma (CName s) = CName s) /\
-   (cnm_temparg_only_inst sigma (TempCall temp args) =
-      TempCall temp (MAP (temparg_inst sigma) args))
-
-     /\
-
-   (* only template arguments *)
-   (nns_inst sigma nns =
-     nns with idents updated_by MAP (cnm_temparg_only_inst sigma))
-
-     /\
-
-   (temparg_inst sigma (TType ty) = TType (type_inst sigma ty)) /\
-   (temparg_inst sigma (TTemp tnm) = TTemp (tempname_inst sigma tnm)) /\
-   (temparg_inst sigma (TVal tva) = TVal (tempval_inst sigma tva))
-
-     /\
-
-   (tempval_inst sigma (TNum i) = TNum i) /\
-   (tempval_inst sigma (TPName s) =
-      case FINDL (\ (p,a). temp_param_name p = s) of
-         NONE -> TPName s
-      || SOME (p,a) -> a) /\
-   (tempval_inst sigma (TObj (nns, objname)) =
-`;
-
-(* instantiate a state_class_info value using a parameters-argument list *)
-val cinfo_inst_def = Define`
-
-  (cinfo_inst sigma ci = <| fields updated_by
-                             MAP (\ (ce,b,p). (centry_inst sigma ce, b, p));
-                            ancestors updated_by
-                             MAP (\ (cs,b,p). (cspec_inst sigma cs, b, p)) |>)
+  (cppid_ty_inst sigma (IDVar s) =
+     case FINDL (\ (p,a). p = TType (TypeID (IDVar s))) sigma of
+        NONE -> Class (IDVar s)
+     || SOME (p, a) -> (case a of TType ty -> ty)) /\
+  (cppid_ty_inst sigma (IDFld cid fld) =
+     Class (IDFld (cppid_inst sigma cid) (sfld_inst sigma fld))) /\
+  (cppid_ty_inst sigma (IDTempCall tempid tempargs) =
+     Class (IDTempCall (tempid_inst sigma tempid)
+                       (MAP (temparg_inst sigma) tempargs))) /\
+  (cppid_ty_inst sigma (IDConstant tnm) = Class (IDConstant tnm))
 
     /\
 
-  (centry_inst sigma (CFnDefn retty nm params body) =
-     CFnDefn (type_inst sigma retty)
-             nm
-             (MAP (\ (nm,ty). (nm, type_inst sigma ty)) params)
-             (stmt_inst sigma body))  /\
-  (centry_inst sigma (FldDecl nm ty) = FldDecl nm (type_inst sigma ty)) /\
+  (cppid_inst sigma cid = dest_class (cppid_ty_inst sigma cid))
+
+    /\
+
+  (temparg_inst sigma (TType ty) = TType (type_inst sigma ty)) /\
+  (temparg_inst sigma (TTemp tid) = TTemp (tempid_inst sigma tid)) /\
+  (temparg_inst sigma (TVal tva) = TVal (temp_valarg_inst sigma tva))
+
+    /\
+
+  (temp_valarg_inst sigma (TNum i) = TNum i) /\
+  (temp_valarg_inst sigma (TObj id) = TObj (cppid_inst sigma id)) /\
+  (temp_valarg_inst sigma (TMPtr id ty) =
+      TMPtr (cppid_inst sigma id) (type_inst sigma ty)) /\
+  (temp_valarg_inst sigma (TVAVar s) =
+      case FINDL (\ (p,a). p = TVal (TVAVar s)) sigma of
+         NONE -> TVAVar s
+      || SOME (p, a) -> (case a of TVal v -> v))
+
+    /\
+
+  (sfld_inst sigma (SFTempCall s targs) =
+             SFTempCall s (MAP (temparg_inst sigma) targs)) /\
+  (sfld_inst sigma (SFName s) = SFName s)
+`
+
+val (type_inst_def, type_inst_ind) = Defn.tprove(type_inst_defn,
+  WF_REL_TAC
+  `measure
+     (\a. case a of
+             INL (_, ty) -> 2 * CPP_Type_size ty
+          || INR (INL (_, id)) -> 2 * CPP_ID_size id
+          || INR (INR (INL (_, id))) -> 2 * CPP_ID_size id + 1
+          || INR (INR (INR (INL (_, targ)))) -> 2 * TemplateArg_size targ
+          || INR (INR (INR (INR (INL (_, tva))))) ->
+               2 * TemplateValueArg_size tva
+          || INR (INR (INR (INR (INR (_, sfld))))) ->
+               2 * StaticField_size sfld)`
+     THEN
+  SRW_TAC [ARITH_ss][] THENL [
+    Induct_on `tylist` THEN SRW_TAC [][] THEN
+    SRW_TAC [ARITH_ss][] THEN FULL_SIMP_TAC (srw_ss() ++ ARITH_ss) [],
+    Induct_on `tempargs` THEN SRW_TAC [][] THEN
+    SRW_TAC [ARITH_ss][] THEN RES_TAC THEN DECIDE_TAC,
+    Induct_on `targs` THEN SRW_TAC [][] THEN
+    SRW_TAC [ARITH_ss][] THEN RES_TAC THEN DECIDE_TAC
+  ]);
+
+val _ = save_thm("type_inst_def", type_inst_def)
+val _ = export_rewrites ["type_inst_def"]
+
+(* instantiate an expression *)
+val expr_inst_def = Define`
+  (expr_inst sigma (Cnum n) = Cnum n) /\
+  (expr_inst sigma (Cchar n) = Cchar n) /\
+  (expr_inst sigma (Cnullptr ty) = Cnullptr (type_inst sigma ty)) /\
+  (expr_inst sigma This = This) /\
+  (expr_inst sigma (Var id) =
+     case id of
+        IDConstant (F,[],s) ->
+           (case FINDL (\ (p,a). p = TVal (TVAVar s)) sigma of
+               NONE -> Var id
+            || SOME (p, a) ->
+                 (case a of
+                     TVal (TNum i) -> Cnum i
+                  || TVal (TObj id') -> Var id'
+                  || TVal (TMPtr cid ty) ->
+                        (case cid of
+                            IDFld cnm fldname -> MemAddr cnm fldname)))
+     || x -> Var id) /\
+  (expr_inst sigma (COr e1 e2) =
+     COr (expr_inst sigma e1) (expr_inst sigma e2)) /\
+  (expr_inst sigma (CAnd e1 e2) =
+     CAnd (expr_inst sigma e1) (expr_inst sigma e2)) /\
+  (expr_inst sigma (CCond e1 e2 e3) =
+     CCond (expr_inst sigma e1) (expr_inst sigma e2) (expr_inst sigma e3)) /\
+  (expr_inst sigma (CApBinary cbop e1 e2) =
+     CApBinary cbop (expr_inst sigma e1) (expr_inst sigma e2)) /\
+  (expr_inst sigma (CApUnary cuop e) = CApUnary cuop (expr_inst sigma e)) /\
+  (expr_inst sigma (Addr e) = Addr (expr_inst sigma e)) /\
+  (expr_inst sigma (Deref e) = Deref (expr_inst sigma e)) /\
+  (expr_inst sigma (MemAddr cid fld) =
+     MemAddr (cppid_inst sigma cid) (sfld_inst sigma fld)) /\
+  (expr_inst sigma (Assign bopopt e1 e2) =
+     Assign bopopt (expr_inst sigma e1) (expr_inst sigma e2)) /\
+  (expr_inst sigma (SVar e fld) = SVar (expr_inst sigma e)
+                                       (sfld_inst sigma fld)) /\
+  (expr_inst sigma (FnApp e args) =
+     FnApp (expr_inst sigma e) (exprl_inst sigma args)) /\
+  (expr_inst sigma (CommaSep e1 e2) =
+     CommaSep (expr_inst sigma e1) (expr_inst sigma e2)) /\
+  (expr_inst sigma (Cast ty e) =
+     Cast (type_inst sigma ty) (expr_inst sigma e)) /\
+  (expr_inst sigma (PostInc e) = PostInc (expr_inst sigma e)) /\
+  (expr_inst sigma (New ty args_opt) =
+     New (type_inst sigma ty) (exprlop_inst sigma args_opt)) /\
+  (expr_inst sigma (CAndOr_sqpt e) = CAndOr_sqpt (expr_inst sigma e)) /\
+  (expr_inst sigma (FnApp_sqpt e args) =
+     FnApp_sqpt (expr_inst sigma e) (exprl_inst sigma args)) /\
+  (expr_inst sigma (LVal ad ty nms) =
+     LVal ad (type_inst sigma ty) (MAP (cppid_inst sigma) nms)) /\
+  (expr_inst sigma (FVal fnid ty eopt) =
+     FVal fnid (type_inst sigma ty) (expropt_inst sigma eopt)) /\
+  (expr_inst sigma (ConstructorFVal b1 b2 ad nm) =
+     ConstructorFVal b1 b2 ad (cppid_inst sigma nm)) /\
+  (expr_inst sigma (ConstructedVal b ad nm) =
+     ConstructedVal b ad (cppid_inst sigma nm)) /\
+  (expr_inst sigma (DestructorCall ad nm) =
+     DestructorCall ad (cppid_inst sigma nm)) /\
+  (expr_inst sigma (RValreq e) = RValreq (expr_inst sigma e)) /\
+  (expr_inst sigma (ECompVal bytes ty) =
+     ECompVal bytes (type_inst sigma ty)) /\
+  (expr_inst sigma (ExceptionExpr e) = ExceptionExpr (expr_inst sigma e)) /\
+
+  (exprl_inst sigma [] = []) /\
+  (exprl_inst sigma (e::es) = expr_inst sigma e :: exprl_inst sigma es) /\
+
+  (exprlop_inst sigma NONE = NONE) /\
+  (exprlop_inst sigma (SOME elist) = SOME (exprl_inst sigma elist)) /\
+
+  (expropt_inst sigma NONE = NONE) /\
+  (expropt_inst sigma (SOME e) = SOME (expr_inst sigma e))
+`
+
+(* this shouldn't ever actually be called, because instantiation shouldn't
+   ever see programs with dynamic helper syntax (such as this) in place *)
+val varlocn_inst_def = Define`
+  (varlocn_inst sigma (RefPlace nopt nm) =
+     RefPlace nopt (cppid_inst sigma nm)) /\
+  (varlocn_inst sigma (ObjPlace n) = ObjPlace n)
+`;
+
+(* fields that are initialised can't be member functions, so there is no
+   chance the MI_fld could be a template call *)
+val meminitid_inst_def = Define`
+  (meminitid_inst sigma (MI_C id) = MI_C (cppid_inst sigma id)) /\
+  (meminitid_inst sigma (MI_fld nm) = MI_fld nm)
+`;
+
+val stmt_inst_defn = Hol_defn "stmt_inst" `
+  (stmt_inst sigma EmptyStmt = EmptyStmt) /\
+  (stmt_inst sigma (CLoop ee st) =
+     CLoop (eexpr_inst sigma ee) (stmt_inst sigma st)) /\
+  (stmt_inst sigma (CIf ee st1 st2) =
+     CIf (eexpr_inst sigma ee) (stmt_inst sigma st1) (stmt_inst sigma st2)) /\
+  (stmt_inst sigma (Standalone ee) = Standalone (eexpr_inst sigma ee)) /\
+  (stmt_inst sigma (Block b vdl stl) =
+     Block b (MAP (vdec_inst sigma) vdl) (MAP (stmt_inst sigma) stl)) /\
+  (stmt_inst sigma (Ret ee) = Ret (eexpr_inst sigma ee)) /\
+  (stmt_inst sigma EmptyRet = EmptyRet) /\
+  (stmt_inst sigma Break = Break) /\
+  (stmt_inst sigma Cont = Cont) /\
+  (stmt_inst sigma (Trap tt st) = Trap tt (stmt_inst sigma st)) /\
+  (stmt_inst sigma (Throw eeopt) =
+     Throw (OPTION_MAP (eexpr_inst sigma) eeopt)) /\
+  (stmt_inst sigma (Catch st handlers) =
+     Catch (stmt_inst sigma st)
+           (MAP (\ (exnpd, st).
+                   ((case exnpd of
+                        NONE -> NONE
+                     || SOME (sopt,ty) -> SOME (sopt, type_inst sigma ty)),
+                    stmt_inst sigma st))
+                handlers)) /\
+  (stmt_inst sigma ClearExn = ClearExn)
+
+     /\
+
+  (eexpr_inst sigma (NormE e se) = NormE (expr_inst sigma e) se) /\
+  (eexpr_inst sigma (EStmt st c) = EStmt (stmt_inst sigma st) c)
+
+     /\
+
+  (vdec_inst sigma (VDec ty nm) =
+     VDec (type_inst sigma ty) (cppid_inst sigma nm)) /\
+  (vdec_inst sigma (VDecInit ty nm init) =
+     VDecInit (type_inst sigma ty)
+              (cppid_inst sigma nm)
+              (initialiser_inst sigma init)) /\
+  (vdec_inst sigma (VDecInitA ty vlocn init) =
+     VDecInitA (type_inst sigma ty)
+               (varlocn_inst sigma vlocn)
+               (initialiser_inst sigma init)) /\
+  (vdec_inst sigma (VStrDec id infoopt) =
+     VStrDec (cppid_inst sigma id) (OPTION_MAP (cinfo_inst sigma) infoopt)) /\
+  (vdec_inst sigma (VException e) = VException (expr_inst sigma e))
+
+     /\
+
+  (centry_inst sigma (CFnDefn ty fld params body) =
+     CFnDefn (type_inst sigma ty)
+             (sfld_inst sigma fld)
+             (MAP (\ (n,ty). (n, type_inst sigma ty)) params)
+             (OPTION_MAP (stmt_inst sigma) body)) /\
+  (centry_inst sigma (FldDecl fldnm ty) =
+     FldDecl fldnm (type_inst sigma ty)) /\
   (centry_inst sigma (Constructor params meminits bodyopt) =
-     Constructor (MAP (\ (nm,ty). (nm, type_inst sigma ty)) params)
-                 (MAP (mem_init_inst sigma) meminits)
+     Constructor (MAP (\ (n,ty). (n, type_inst sigma ty)) params)
+                 (MAP (\ (mid,optargs). (meminitid_inst sigma mid,
+                                         OPTION_MAP (MAP (expr_inst sigma))
+                                                    optargs))
+                      meminits)
                  (OPTION_MAP (stmt_inst sigma) bodyopt)) /\
   (centry_inst sigma (Destructor bodyopt) =
      Destructor (OPTION_MAP (stmt_inst sigma) bodyopt))
 
-    /\
+     /\
 
+  (cinfo_inst sigma ci =
+     <| fields := MAP (\ (ce,b,p). (centry_inst sigma ce, b, p)) ci.fields;
+        ancestors := MAP (\ (cs,b,p). (cppid_inst sigma cs, b, p))
+                         ci.ancestors |>)
+
+     /\
+
+  (initialiser_inst sigma (DirectInit0 elist) =
+     DirectInit0 (MAP (expr_inst sigma) elist)) /\
+  (initialiser_inst sigma (DirectInit ee) =
+     DirectInit (eexpr_inst sigma ee)) /\
+  (initialiser_inst sigma (CopyInit ee) = CopyInit (eexpr_inst sigma ee))
 `;
 
-val mk_inst_def = Define`
-  (mk_inst [] args = []) /\ (* args will always be empty at this point *)
-  (mk_inst ((p, dflt) :: prest) (a::args) =
-     (p, a) :: mk_inst (inst_inst p a prest) args)  /\
-  (mk_inst ((p,dflt) :: prest) [] =
-     (p, THE dflt) :: mk_inst (inst_inst [(p,THE dflt)] prest) []) /\
+val size_def = DB.fetch "statements" "CStmt_size_def"
+val _ = augment_srw_ss [rewrites [size_def]]
 
-  (inst_inst p a [] = []) /\
-  (inst_inst p a (pm::pms) = inst_inst1 p a pm :: inst_inst p a pms) /\
-
-  (inst_inst1 (TempType p) (TType ty) (TempType p', NONE) =
-     (TempType p', NONE)) /\
-  (inst_inst1 (TempType p) (TType ty) (TempType p', SOME (TType ty')) =
-     (TempType p', SOME (TType (type_inst [(TempType p, TType ty)] ty')))) /\
-  (inst_inst1 (TempType p) (TType ty) (TempParam ty' n, NONE) =
-     (TempParam (type_inst [(TempType p, TType ty)] ty') n, NONE)) /\
-  (inst_inst1 (TempType p) (TType ty) (TempParam ty' n, SOME (TVal tval)) =
-     (TempParam (type_inst [(TypeType p, TType ty)] ty') n,
-      SOME (TVal (inst_tval
-
-`;
+val (stmt_inst_def, stmt_inst_ind) = Defn.tprove(
+  stmt_inst_defn,
+  WF_REL_TAC
+    `measure
+      (\s.
+        case s of
+           INL (_, st) -> CStmt_size st
+        || INR (INL (_, ee)) -> ExtE_size ee
+        || INR (INR (INL (_, vd))) -> var_decl_size vd
+        || INR (INR (INR (INL (_, ce)))) -> class_entry_size ce
+        || INR (INR (INR (INR (INL (_, ci))))) -> class_info_size ci
+        || INR (INR (INR (INR (INR (_, i))))) -> initializer_size i)` THEN
+  SRW_TAC [ARITH_ss][] THENL [
+    Induct_on `handlers` THEN SRW_TAC [][] THEN SRW_TAC [ARITH_ss][] THEN
+    RES_TAC THEN DECIDE_TAC,
+    Induct_on `vdl` THEN SRW_TAC [][] THEN SRW_TAC [ARITH_ss][] THEN
+    RES_TAC THEN DECIDE_TAC,
+    Cases_on `ci` THEN FULL_SIMP_TAC (srw_ss()) [] THEN
+    Induct_on `l` THEN SRW_TAC [][] THEN SRW_TAC [ARITH_ss][] THEN
+    RES_TAC THEN DECIDE_TAC,
+    Induct_on `stl` THEN SRW_TAC [][] THEN SRW_TAC [ARITH_ss][] THEN
+    RES_TAC THEN DECIDE_TAC
+  ]);
 
 
 val cinfo_def = Define`
-  cinfo s ((ns, nm) : class_spec) : class_info =
-     case nm of
-        CName s -> FST (THE (s.classmap ' (ns,nm)))
-     || TempCall s args ->
-          let (params,info0) = s.class_templates ' (ns,s) in
-          let info1 = FST (THE info0) in
-          let inst = inst_inst params args in
-          in
-              cinfo_inst inst info1
+  cinfo s cnm : class_info = FST (THE (s.classmap ' cnm))
 `;
 
 (* set of a state's fully defined class *)
@@ -372,20 +515,26 @@ val path_via_def = Define`
 
 (* finding fields W et al. 5.1.3
    - omitting constructors and destructors as these can't be called normally *)
+val SFld_to_ID_def = Define`
+  (SFld_to_ID (SFTempCall s args) = IDTempCall (TemplateConstant (F,[],s))
+                                               args) /\
+  (SFld_to_ID (SFName s) = Base s)
+`;
+
 val fieldname_def = Define`
-  (fieldname (FldDecl n ty) = n) /\
+  (fieldname (FldDecl fldnm ty) = SFName fldnm) /\
   (fieldname (CFnDefn retty n args body) = n)
 `
 
 (* again, omitting constructors and destructors as these can't be called *)
 val fieldtype_def = Define`
-  (fieldtype (FldDecl n ty) = ty) /\
+  (fieldtype (FldDecl fld ty) = ty) /\
   (fieldtype (CFnDefn retty n args body) = Function retty (MAP SND args))
 `;
 
 (* those fields for which the above two predicates are well-defined *)
 val okfield_def = Define`
-  (okfield (FldDecl n ty) = T) /\
+  (okfield (FldDecl fld ty) = T) /\
   (okfield (CFnDefn retty n args body) = T) /\
   (okfield _ = F)
 `;
@@ -546,8 +695,8 @@ val nsdmembers_def = Define`
         (mapPartial
            (\ce. case ce of
                     (CFnDefn ret nm args bod, stat, prot) -> NONE
-                 || (FldDecl nm ty, stat, prot) -> if stat then NONE
-                                                   else SOME (nm,ty)
+                 || (FldDecl fld ty, stat, prot) -> if stat then NONE
+                                                    else SOME (fld,ty)
                  || _ -> NONE)
            (cinfo s c).fields)
     else NONE
@@ -730,7 +879,7 @@ val subobj_offset_def = Define`
 val expr_type_comps_def = Define`
   expr_type_comps s =
     <| class_fields :=
-          FUN_FMAP (\c. THE (nsdmembers s c))
+          FUN_FMAP (\c. MAP (\ (n,ty). (SFName n, ty)) (THE (nsdmembers s c)))
                    { c | ?v. c IN FDOM s.classmap /\
                              (s.classmap ' c = SOME v) };
        var_types := s.typemap ;
@@ -749,7 +898,11 @@ val MEM_splits = prove(
 val hasfld_imp_lfi = store_thm(
   "hasfld_imp_lfi",
   ``s |- C has least fld -: ftype via p' /\ object_type ftype ==>
-    ?i. lookup_field_info (THE (nsdmembers s (LAST p'))) fld (i,ftype)``,
+    ?i. lookup_field_info
+          (MAP (\ (n,ty). (SFName n, ty))
+               (THE (nsdmembers s (LAST p'))))
+          fld
+          (i,ftype)``,
   SRW_TAC [][fieldty_via_def, FieldDecls_def, nsdmembers_def] THEN
   Cases_on `centry` THEN
   FULL_SIMP_TAC (srw_ss()) [fieldtype_def, typesTheory.object_type_def,
