holsrcs/sanityScript.sml
@@ -27,27 +27,29 @@ val _ = new_theory "sanity";
    ---------------------------------------------------------------------- *)
 
 open side_effectsTheory
-val val2mem_fnmap = store_thm(
-  "val2mem_fnmap",
+val val2mem_fnmap0 = prove(
   ``(val2mem s a v).fnmap = s.fnmap``,
   SRW_TAC [][statesTheory.val2mem_def]);
+val val2mem_fnmap = save_thm(
+  "val2mem_fnmap",
+  SIMP_RULE (srw_ss()) [] val2mem_fnmap0)
 val _ = export_rewrites ["val2mem_fnmap"]
-val apply_se_preserves_fnmaps = prove(
+val apply_se_preserves_fnmaps = SIMP_RULE (srw_ss()) [] (prove(
   ``apply_se (se0,s0) (se,s) ==> (s0.fnmap = s.fnmap)``,
     SRW_TAC [][apply_se_def, apply_lse_def] THEN
     Cases_on `ise` THEN
-    FULL_SIMP_TAC (srw_ss()) [se_on_state_def])
+    FULL_SIMP_TAC (srw_ss()) [se_on_state_def]))
 
-val vdeclare_preserves_fnmaps = prove(
+val vdeclare_preserves_fnmaps = SIMP_RULE (srw_ss()) [] (prove(
   ``vdeclare s0 ty name s ==> (s0.fnmap = s.fnmap)``,
-  SRW_TAC [][vdeclare_def] THEN SRW_TAC [][]);
+  SRW_TAC [][vdeclare_def] THEN SRW_TAC [][]));
 
 val declmng_preserves_fnmaps = prove(
   ``(!ee0 s0 see. mng ee0 s0 see ==> (s0.fnmap = (FST see).fnmap)) /\
     (!s. (vdf s).fnmap = s.fnmap) ==>
     !d0s0 ds. declmng mng vdf d0s0 ds ==>
               ((SND d0s0).fnmap = (SND ds).fnmap)``,
-  STRIP_TAC THEN HO_MATCH_MP_TAC declmng_ind THEN
+  SIMP_TAC (srw_ss()) [] THEN STRIP_TAC THEN HO_MATCH_MP_TAC declmng_ind THEN
   SRW_TAC [][] THEN
   TRY (METIS_TAC [lval2rval_states_equal, apply_se_preserves_fnmaps,
                   vdeclare_preserves_fnmaps]) THEN
